unusedglob/VerComp.v
@@ -8,6 +8,7 @@ Require Import Integers.
 Require Import Memory.
 Require Import Smallstep.
 Require Import Inject InjectFootprint.
+Require Import CKLRAlgebra.
 Require Import Callconv ForwardSim.
 
 (** * Test1: compose injp' ⋅ injp' = injp' *)
@@ -21,11 +22,11 @@ L1 <= injp'-> injp' L3
 Section COMPOSE_FORWARD_SIMULATIONS.
 
 Context (L1: semantics li_c li_c) (L2: semantics li_c li_c) (L3: semantics li_c li_c).
-
+(*
 Definition symtbl_dom (se: Genv.symtbl) : meminj :=
   fun b => if Mem.sup_dec b (Genv.genv_sup se) then Some (b,0)
         else None.
-
+*)
 Definition source_inj (se: Genv.symtbl) (f : meminj) :=
   fun b => if Mem.sup_dec b (Genv.genv_sup se) then
         Some (b,0) else meminj_dom f b.
@@ -204,32 +205,202 @@ Proof.
   - reflexivity.
 Qed.
 
-Lemma mem_inject_source : forall f m1 m2 se,
-    Mem.inject f m1 m2 ->
-    Mem.inject (source_inj se f) m1 m1.
-Proof.
-  intros.
-  exploit mem_inject_dom; eauto.
-  intro.
-  Search Mem.inject.
-Definition soucr_world (w: injp_world) (se:Genv.symtbl) :=
-  match w with
-  |injpw f m1 m2 Hm =>
-     injpw (source_inj se f) m1 m1 (mem_inject_dom f m1 m2 Hm)
-  end.
+Definition source_world f m1 m2 (Hm: Mem.inject f m1 m2) (se:Genv.symtbl) (Hse: Mem.sup_include (Genv.genv_sup se) (Mem.support m1)) :=
+     injpw (source_inj se f) m1 m1 (mem_source_inj se f m1 m2 Hse Hm).
 
 Lemma match_stbls_dom' f se1 se2:
   Genv.match_stbls' f se1 se2 ->
-  Genv.match_stbls (meminj_dom f) se1 se1.
+  Genv.match_stbls (source_inj se1 f) se1 se1.
 Proof.
-  intros Hse. unfold meminj_dom. split; eauto; intros.
-  - inv Hse.
-  - inv Hse. admit
-  - destruct (f b1) as [[xb2 xdelta] | ] eqn:Hb; inv H. reflexivity.
-  - destruct (f b1) as [[xb2 xdelta] | ] eqn:Hb; inv H. reflexivity.
-  - destruct (f b1) as [[xb2 xdelta] | ] eqn:Hb; inv H. reflexivity.
+  intros Hse. unfold source_inj. unfold meminj_dom. split; eauto; intros.
+  - destruct Mem.sup_dec; try congruence. eauto.
+  - inv Hse. exists b2. destruct Mem.sup_dec; try congruence.
+  - destruct Mem.sup_dec. inv H. reflexivity.
+    destruct (f b1) as [[xb2 xdelta] | ] eqn:Hb; inv H. reflexivity.
+  - destruct Mem.sup_dec. inv H. reflexivity.
+    destruct (f b1) as [[xb2 xdelta] | ] eqn:Hb; inv H. reflexivity.
+  - destruct Mem.sup_dec. inv H. reflexivity.
+    destruct (f b1) as [[xb2 xdelta] | ] eqn:Hb; inv H. reflexivity.
 Qed.
 
+Lemma compose_meminj_midvalue: forall j1 j2 v1 v3,
+    Val.inject (compose_meminj j1 j2) v1 v3 ->
+    exists v2, Val.inject j1 v1 v2 /\ Val.inject j2 v2 v3.
+Proof.
+  intros. inv H.
+  eexists. split; econstructor; eauto.
+  eexists. split; econstructor; eauto.
+  eexists. split; econstructor; eauto.
+  eexists. split; econstructor; eauto.
+  unfold compose_meminj in H0.
+  destruct (j1 b1) as [[b2' d1]|] eqn:M1; try congruence.
+  destruct (j2 b2') as [[b3' d2]|] eqn:M2; inv H0.
+  eexists. split. econstructor; eauto.
+  econstructor; eauto. rewrite add_repr.
+  rewrite Ptrofs.add_assoc. auto.
+  exists Vundef. split; constructor.
+Qed.
+
+
+Lemma compose_fsim_components_old_new:
+  fsim_components (cc_c injp) (cc_c injp) L1 L2 ->
+  fsim_components' (cc_c' injp') (cc_c' injp') L2 L3 ->
+  fsim_components' (cc_c' injp') (cc_c' injp') L1 L3.
+  intros [index order match_states Hsk props order_wf].
+  intros [index' order' match_states' Hsk' props' order_wf'].
+  set (ff_index := (index' * index)%type).
+  set (ff_order := lex_ord (clos_trans _ order') order).
+  (*How to construct w1 here? add the well-form condition into fsim_components *)
+  set (ff_match_states :=
+         fun se1 se3 (w: injp_world) (i: ff_index) (s1: state L1) (s3: state L3) =>
+           exists s2 w12 w23,
+             match_states se1 se1 w12 (snd i) s1 s2 /\
+             match_states' se1 se3 w23 (fst i) s2 s3 /\
+               match_senv (cc_c injp) w12 se1 se1 /\
+               match_senv' (cc_c' injp') w23 se1 se3 /\
+               forall r1 r2 r3, match_reply (cc_c injp) w12 r1 r2 /\
+                             match_reply' (cc_c' injp') w23 r2 r3 ->
+                           match_reply' (cc_c' injp') w r1 r3).
+  apply Forward_simulation' with ff_order ff_match_states.
+  3: { unfold ff_order. auto using wf_lex_ord, wf_clos_trans. }
+  1: { congruence. }
+  intros se1 se2 w Hse2 Hcompat. cbn in *.
+  destruct w as [j m1 m2 Hm]. inversion Hse2. subst.
+  set (w1 := source_world j m1 m2 Hm se1 H5).
+  assert (Hse1: injp_match_stbls w1 se1 se1).
+  { constructor; eauto.
+    eapply  match_stbls_dom'; eauto.
+  }
+  assert (Hvalid1: Genv.valid_for (skel L1) se1).
+  {
+    inv Hcompat. eauto.
+  }
+  rewrite Hsk in Hcompat.
+  (* exploit props; eauto. intros Fsim1.*)
+  (* exploit props'; eauto. intros Fsim2. *)
+  split.
+- (* valid query *)
+  intros q1 q3 Hq13.
+  assert (match_query (cc_c injp) w1 q1 q1).
+  {
+    unfold w1. inv Hq13. cbn in *. inv H1. constructor; cbn in *.
+    eapply val_inject_dom; eauto.
+    eapply val_inject_list_dom; eauto.
+    econstructor; eauto. eauto.
+  }
+  etransitivity.
+  eapply fsim_match_valid_query'; eauto.
+  eapply fsim_match_valid_query; eauto.
+- (* initial states *)
+  intros q1 q3 s1 Hq13 Hs1.
+  assert (match_query (cc_c injp) w1 q1 q1).
+  {
+    unfold w1. inv Hq13. cbn in *. inv H1. constructor; cbn in *.
+    eapply val_inject_dom; eauto.
+    eapply val_inject_list_dom; eauto.
+    econstructor; eauto. eauto.
+  }
+  edestruct (@fsim_match_initial_states) as (i & s2 & A & B); eauto.
+  edestruct (@fsim_match_initial_states') as (i' & s3 & C & D); eauto.
+  exists (i', i); exists s3; split; auto. exists s2; eauto.
+  intuition eauto.
+  admit. (*TODO, compose proof in Injectfootprint and the oracle*)
+- (* final states *)
+  intros. destruct H as (s3 & w12 & w23 & A & B & C & D & E).
+  edestruct (@fsim_match_final_states) as (r2 & Hr2 & Hr12); eauto.
+  edestruct (@fsim_match_final_states') as (r3 & Hr3 & Hr23); eauto.
+  exists r3. split. eauto. eapply E. split. eapply Hr12. eauto.
+- (* external states *)
+  intros. destruct H as (s3 & w12 & w23 & A & B & C & D & E).
+  edestruct (@fsim_match_external) as (w12A & q2 & Hq2 & Hq12 & Hw12 & Hk12); eauto.
+  edestruct (@fsim_match_external') as (w23A & q3 & Hq3 & Hq23 & Hw23 & Hk23); eauto.
+  {
+    cbn in *. destruct w12A as [j12 m1' m2' Hm12'].
+    inv Hq12. cbn in *. inv H3. rename m0 into m1'. rename m3 into m2'.
+    destruct w23A as [j23 m2'' m3' Hm23'].
+    inv Hq23. cbn in *. inv H13. rename m3 into m3'.
+    exists (injpw (compose_meminj j12 j23) m1' m3' (Mem.inject_compose _ _ _ _ _ Hm4 Hm7)).
+    exists (cq vf3 sg vargs3 m3').
+    repeat apply conj; eauto.
+    - (*match_query*)
+      econstructor; cbn; eauto. eapply val_inject_compose; eauto.
+      eapply val_inject_list_compose; eauto.
+    - (*match_stbls'*)
+      clear - Hw23 Hw12. cbn in *. inv Hw12. inv Hw23.
+      constructor; eauto.
+      eapply Genv.match_stbls_stbls'_compose; eauto.
+    - (*after_external*)
+      cbn.
+      intros r1 r3 s1' [w13' [Hw Hr13]] Hafter.
+      inv Hr13. inv H7. cbn in *. rename f into j13'. rename Hm11 into INJ13'.
+      cbn in Hw. rename m1'0 into m1'A. rename m2'0 into m3'A.
+      rename m1' into m1A. rename m2' into m2A. rename m3' into m3A.
+      rename Hm4 into INJ12. rename Hm7 into INJ23.
+      inversion Hw as [? ? ? ? ? ? ? ? RO1 RO3 MAXPERM1 MAXPERM3 UNCHANGE1 UNCHANGE3 INCR13 DISJ13]. subst.
+      generalize (inject_implies_image_in _ _ _ INJ12).
+      intros IMGIN12.
+      generalize (inject_implies_image_in _ _ _ INJ23).
+      intros IMGIN23.
+      generalize (inject_implies_dom_in _ _ _ INJ12).
+      intros DOMIN12.
+      generalize (inject_implies_dom_in _ _ _ INJ23).
+      intros DOMIN23.
+      generalize (inject_implies_dom_in _ _ _ INJ13').
+      intros DOMIN13'.
+      generalize (Mem.unchanged_on_support _ _ _ UNCHANGE1).
+      intros SUPINCL1.
+      generalize (Mem.unchanged_on_support _ _ _ UNCHANGE3).
+      intros SUPINCL3.
+      generalize (inject_incr_inv _ _ _ _ _ _ _ DOMIN12 IMGIN12 DOMIN23 DOMIN13' SUPINCL1 INCR13 DISJ13).
+      intros (j12' & j23' & m2'_sup & JEQ & INCR12 & INCR23 & SUPINCL2 & DOMIN12' & IMGIN12' & DOMIN23' & INCRDISJ12 & INCRDISJ23 & INCRNOLAP & ADDZERO & ADDEXISTS & ADDSAME).
+      subst. cbn in *.
+      set (m2'A := m2' m1A m2A m1'A j12 j23 j12' m2'_sup INJ12 ).
+      assert (INJ12' :  Mem.inject j12' m1'A m2'A). eapply INJ12'; eauto.
+      assert (INJ23' :  Mem.inject j23' m2'A m3'A). eapply INJ23'; eauto.
+      set (w12' := injpw j12' m1'A m2'A INJ12').
+      set (w23' := injpw j23' m2'A m3'A INJ23').
+      rename vres2 into vres3.
+      exploit compose_meminj_midvalue; eauto.
+      intros [vres2 [RES1 RES2]].
+      assert (UNC21:Mem.unchanged_on (loc_out_of_reach j12 m1A) m2A m2'A).
+      eapply UNCHANGE21; eauto.
+      (* end of injp decomposition *)
+      set (r2 := cr vres2 m2'A ).
+      edestruct Hk12 as (i12' & s2' & Hs2' & Hs12'); eauto.
+      instantiate (1:= r2).
+      exists w12'. split. constructor; eauto. eapply ROUNC2; eauto.
+      eapply MAXPERM2; eauto.
+      eapply Mem.unchanged_on_implies; eauto.
+      intros. red. unfold compose_meminj.
+      rewrite H7. reflexivity.
+      constructor; eauto. constructor; eauto.
+      edestruct Hk23 as (i23' & s3' & Hs3' & Hs23'); eauto.
+      instantiate (1:= (cr vres3 m3'A)). exists w23'.
+      split. constructor; eauto. eapply ROUNC2; eauto.
+      eapply MAXPERM2; eauto.
+      eapply UNCHANGE22; eauto. eapply out_of_reach_trans; eauto.
+      constructor; eauto. constructor.
+      exists (i23', i12'), s3'. split; auto. exists s2', w12, w23; eauto.
+  }
+- (* simulation *)
+  intros. destruct H0 as (s3 & w12 & w23 & MS1 & MS2 & MENV1 & MENV2 & RESULT).
+  destruct i as [i2 i1]; simpl in *.
+  edestruct (@fsim_simulation') as [(i1' & s3' & C & D) | (i1' & C & D & E)]; eauto.
++ (* L2 makes one or several steps. *)
+  edestruct (@simulation_plus') as [(i2' & s2' & P & Q) | (i2' & P & Q & R)]; eauto.
+* (* L3 makes one or several steps *)
+  exists (i2', i1'); exists s2'; split. auto. exists s3', w12, w23; auto.
+* (* L3 makes no step *)
+  exists (i2', i1'); exists s2; split.
+  right; split. subst t; apply star_refl. red. left. auto.
+  exists s3', w12, w23; auto.
++ (* L2 makes no step *)
+  exists (i2, i1'); exists s2; split.
+  right; split. subst t; apply star_refl. red. right. auto.
+  exists s3, w12, w23; auto.
+Admitted.
+
+(*
 Lemma compose_fsim_components':
   fsim_components' (cc_c' injp') (cc_c' injp') L1 L2 ->
   fsim_components' (cc_c' injp') (cc_c' injp') L2 L3 ->
@@ -257,7 +428,6 @@ Proof.
   }
   assert (Hse1: Genv.valid_for (skel L1) se1).
   {}
-  Search Genv.skel_le.
   { rewrite <- Hsk. eapply match_senv_valid_for; eauto. }
   constructor.
 - (* valid query *)
@@ -298,14 +468,14 @@ Proof.
   right; split. subst t; apply star_refl. red. right. auto.
   exists s3; auto.
 Qed.
-
-Lemma compose_forward_simulations:
-  forward_simulation ccA12 ccB12 L1 L2 ->
-  forward_simulation ccA23 ccB23 L2 L3 ->
-  forward_simulation (ccA12 @ ccA23) (ccB12 @ ccB23) L1 L3.
+*)
+Lemma compose_forward_simulations_old_new:
+  forward_simulation (cc_c injp) (cc_c injp) L1 L2 ->
+  forward_simulation' (cc_c' injp') (cc_c' injp') L2 L3 ->
+  forward_simulation' (cc_c' injp') (cc_c' injp') L1 L3.
 Proof.
   intros [X] [Y]. constructor.
-  apply compose_fsim_components; auto.
+  apply compose_fsim_components_old_new; auto.
 Qed.
 
 End COMPOSE_FORWARD_SIMULATIONS.
